"A princess is as old as the prince will be when the princess is twice as old as the prince was when the princess' age was half the sum of their present age."

A princess is as old (S) as the prince will be (P_future) when the princess is twice as old (S_future) as the prince was (P_past) when the princess' age was (S_past) half the sum of their present age (P+S).

1) S_past = (P + S)/2

2) P_past = S_past + (P-S)

3) S_future = 2 * P_past

4) P_future = S_future + (P-S)

5) S = P_future



#### ####



Start 5)

S = P_future



.4) -> 5)

  S = S_future + (P-S)



.3) -> 5)

  S = 2P_past + (P - S)
  
  
  
.2) -> 5)

  S = 2(S_past + (P - S)) + (P - S)
  
  
  
.1) -> 5)

  S = 2[ ((P + S)/2) + (P - S) ] + (P - S)
  
  
  
# Simplify
S = (2/2)(P + S) + 2(P - S) + (P - S)

S = P + S + (2)P - (2)S + P -S

S = (4)P - (2)S

(3)S = (4)P

S = (4/3)P



The Princess (S) is 4/3 the age of the Prince (P).
